fix theorems

Cslib/Logics/IPL/NJ/Basic.lean
@@ -3,323 +3,447 @@ Copyright (c) 2025 Thomas Waring. All rights reserved.
 Released under Apache 2.0 license as described in the file LICENSE.
 Authors: Thomas Waring
 -/
-import Cslib.Logics.IPL.NJ.Defs
+import Mathlib.Data.Finset.Insert
+import Mathlib.Data.Finset.SDiff
 
-/-! # Elementary derivations and equivalences in NJ -/
+/-!
+# Gentzen's NJ
+
+Natural deduction for intuitionistic propositional logic.
+
+## Main definitions
+
+- `Proposition` : a type of propositions with atoms in a given type.
+- `Derivation` :  natural deduction derivation, done in "sequent style", ie with explicit
+hypotheses at each step. Contexts are `Finset`'s of propositions, which avoids explicit contraction
+and exchange, and the axiom rule derives `{A} ∪ Γ ⊢ A` for any context `Γ`, allowing weakening to
+be a derived rule.
+- `Derivable` : defined as `Nonempty (Derivation S)`.
+- `Proposition.equiv` and `Proposition.Equiv` : `Type`- and `Prop`-valued equivalence of
+propositions.
+
+## Main results
+
+- `Derivation.weak` : weakening as a derived rule.
+- `Derivation.subs` : substituting a derivation for a hypothesis.
+- `equiv_equivalence` : equivalence of propositions is an equivalence.
+
+## References
+
+- Dag Prawitz, *Natural Deduction: a proof-theoretical study*.
+- The sequent-style natural deduction I present here doesn't seem to be common, but it is tersely
+presented in §10.4 of Troelstra & van Dalen's *Constructivism in Mathematics: an introduction*.
+(Suggestions of better references welcome!)
+-/
+
+universe u
 
 variable {Atom : Type u} [DecidableEq Atom]
 
 namespace IPL
 
-open Proposition
+/-- Propositions. We view negation as a defined connective ~A := A → ⊥ -/
+inductive Proposition (Atom : Type u) : Type u where
+  /-- Propositional atoms -/
+  | atom (x : Atom)
+  /-- Falsum -/
+  | bot
+  /-- Conjunction -/
+  | conj (a b : Proposition Atom)
+  /-- Disjunction -/
+  | disj (a b : Proposition Atom)
+  /-- Implication -/
+  | impl (a b : Proposition Atom)
+deriving DecidableEq, BEq
 
 namespace NJ
 
+open Proposition
+
+/-- Contexts are finsets of propositions. -/
+abbrev Ctx (Atom) := Finset (Proposition Atom)
+
+/-- Theories are abitrary sets of propositions. -/
+abbrev Theory (Atom) := Set (Proposition Atom)
+
+abbrev Theory.empty (Atom) : Theory (Atom) := ∅
+
+/-- Sequents {A₁, ..., Aₙ} ⊢ B. -/
+abbrev Sequent (Atom) := Ctx Atom × Proposition Atom
+
+/-- A derivation of {A₁, ..., Aₙ} ⊢ B demonstrates B using (undischarged) assumptions among Aᵢ. -/
+inductive Derivation : Sequent Atom → Type _ where
+  /-- Axiom (or assumption) -/
+  | ax (Γ : Ctx Atom) (A : Proposition Atom) : Derivation ⟨insert A Γ, A⟩
+  /-- Falsum elimination (ex falso quodlibet) -/
+  | botE {Γ : Ctx Atom} (A : Proposition Atom) : Derivation ⟨Γ, bot⟩ → Derivation ⟨Γ, A⟩
+  /-- Conjunction introduction -/
+  | conjI {Γ : Ctx Atom} {A B : Proposition Atom} :
+      Derivation ⟨Γ, A⟩ → Derivation ⟨Γ, B⟩ → Derivation ⟨Γ, conj A B⟩
+  /-- Conjunction elimination left -/
+  | conjE₁ {Γ : Ctx Atom} {A B : Proposition Atom} : Derivation ⟨Γ, conj A B⟩ → Derivation ⟨Γ, A⟩
+  /-- Conjunction elimination right -/
+  | conjE₂ {Γ : Ctx Atom} {A B : Proposition Atom} : Derivation ⟨Γ, conj A B⟩ → Derivation ⟨Γ, B⟩
+  /-- Disjunction introduction left -/
+  | disjI₁ {Γ : Ctx Atom} {A B : Proposition Atom} : Derivation ⟨Γ, A⟩ → Derivation ⟨Γ, disj A B⟩
+  /-- Disjunction introduction right -/
+  | disjI₂ {Γ : Ctx Atom} {A B : Proposition Atom} : Derivation ⟨Γ, B⟩ → Derivation ⟨Γ, disj A B⟩
+  /-- Disjunction elimination -/
+  | disjE {Γ : Ctx Atom} {A B C : Proposition Atom} : Derivation ⟨Γ, disj A B⟩ →
+      Derivation ⟨insert A Γ, C⟩ → Derivation ⟨insert B Γ, C⟩ → Derivation ⟨Γ, C⟩
+  /-- Implication introduction -/
+  | implI {A B : Proposition Atom} (Γ : Ctx Atom) :
+      Derivation ⟨insert A Γ, B⟩ → Derivation ⟨Γ, impl A B⟩
+  /-- Implication elimination -/
+  | implE {Γ : Ctx Atom} {A B : Proposition Atom} :
+      Derivation ⟨Γ, impl A B⟩ → Derivation ⟨Γ, A⟩ → Derivation ⟨Γ, B⟩
+
+inductive Theory.Derivable (T : Theory Atom) (A : Proposition Atom) : Prop
+  | der (Γ : Ctx Atom) (hΓ : ↑Γ ⊆ T) (D : Derivation ⟨Γ, A⟩) : T.Derivable A
+
+theorem Theory.Derivable.theory_weak (T T' : Theory Atom) (hT : T ⊆ T') (A : Proposition Atom) :
+    T.Derivable A → T'.Derivable A
+  | .der Γ hΓ D => ⟨Γ, fun ⦃_⦄ a_1 => hT (hΓ a_1), D⟩
+
+/-- A sequent is derivable if it has a derivation. -/
+abbrev Theory.SDerivable (T : Theory Atom) (S : Sequent Atom) := Theory.Derivable (T ∪ ↑S.1) S.2
+
+theorem Theory.SDerivable.theory_weak (T T' : Theory Atom) (hT : T ⊆ T') (S : Sequent Atom) :
+    T.SDerivable S → T'.SDerivable S
+  | .der Γ hΓ D => ⟨Γ, by grind, D⟩
+
+/-- A proposition is derivable if it has a derivation from the empty context. -/
+abbrev Derivable : Proposition Atom → Prop := Theory.empty Atom |>.Derivable
+
+abbrev SDerivable : Sequent Atom → Prop := Theory.empty Atom |>.SDerivable
+
+theorem derivable_iff {A : Proposition Atom} : Derivable A ↔ Nonempty (Derivation ⟨∅, A⟩) := by
+  constructor
+  · intro ⟨Γ, hΓ, D⟩
+    exact Finset.eq_empty_of_forall_notMem hΓ ▸ ⟨D⟩
+  · intro ⟨D⟩
+    refine ⟨∅, by simp, D⟩
+
+/-- An equivalence between A and B is a derivation of B from A and vice-versa. -/
+def Proposition.equiv (A B : Proposition Atom) := Derivation ⟨{A},B⟩ × Derivation ⟨{B},A⟩
+
+def Theory.Equiv (T : Theory Atom) (A B : Proposition Atom) :=
+  T.Derivable (A.impl B) ∧ T.Derivable (B.impl A)
+
+/-- Two propositions A and B are equivalent if B can be derived from A and vice-versa. -/
+abbrev Equiv : Proposition Atom → Proposition Atom → Prop := Theory.empty Atom |>.Equiv
+
 open Derivation
 
-/-!
-### Negation theorems
+/-- A fixed choice of a derivable proposition (of course any two are equivalent). -/
+def Proposition.top : Proposition Atom := impl bot bot
 
-The following are valid in minimal logic, so we use `impl (-) C` over `~(-) := impl (-) bot`.
--/
+def derivationTop : Derivation (Atom := Atom) ⟨∅, Proposition.top⟩ :=
+  implI ∅ <| ax (Atom := Atom) ∅ bot
 
-/-- Double negation introduction -/
-def Derivation.dni {A B : Proposition Atom} : Derivation ⟨{A}, impl (impl A B) B⟩ :=
-  implI (A := A.impl B) _ <|
-  implE (A := A) (ax' (by grind)) (ax' (by grind))
+theorem Theory.top_derivable (T : Theory Atom) : T.Derivable Proposition.top := by
+  refine ⟨∅, by simp, derivationTop⟩
 
-theorem Derivable.dni {A B : Proposition Atom} : Derivable ⟨{A},impl (impl A B) B⟩ :=
-  ⟨Derivation.dni⟩
+theorem top_derivable : Derivable (Atom := Atom) Proposition.top :=
+  Theory.top_derivable (Theory.empty Atom)
 
-/-- The double negation of excluded-middle, or in minimal-logic-style ⊢ (A ∨ (A → B)) → B → B. -/
-def Derivation.notNotLEM {A B : Proposition Atom} :
-    Derivation ⟨∅, (A.disj <| impl A B).impl B |>.impl B⟩ :=
-  implI _ <|
-  implE (A := A.disj (A.impl B)) (ax' <| by grind) <|
-  disjI₂ <|
-  implI _ <|
-  implE (A := A.disj (A.impl B)) (ax' <| by grind) <|
-  disjI₁ <|
-  ax' <| by grind
+/-! ### Common proof patterns -/
 
-theorem Derivable.not_not_lem {A B : Proposition Atom} :
-    Derivable ⟨∅, (A.disj <| impl A B).impl B |>.impl B⟩ := ⟨Derivation.notNotLEM⟩
+/-- A convenient reformulation of the axiom rule. -/
+def Derivation.ax' {Γ : Ctx Atom} {A : Proposition Atom} (h : A ∈ Γ) : Derivation ⟨Γ,A⟩ := by
+  have : Γ = insert A Γ := by grind
+  rw [this]
+  apply ax
 
-/-- Triple negation elimination -/
-def Derivation.tne {A B : Proposition Atom} :
-    Derivation ⟨{((A.impl B).impl B).impl B}, A.impl B⟩ :=
-  implI _ <|
-  implE (A := (A.impl B).impl B) (ax' <| by grind) <|
-  Derivation.dni.weak' (Γ := {A}) (by grind)
+/-- Weakening is a derived rule. -/
+def Derivation.weak {Γ : Ctx Atom} {A : Proposition Atom} (Δ : Ctx Atom) :
+    (D : Derivation ⟨Γ, A⟩) → Derivation ⟨Γ ∪ Δ, A⟩
+  | ax Γ A => (Finset.insert_union A Γ Δ) ▸ ax (Γ ∪ Δ) A
+  | botE A D => botE A <| D.weak Δ
+  | conjI D D' => conjI (D.weak Δ) (D'.weak Δ)
+  | conjE₁ D => conjE₁ <| D.weak Δ
+  | conjE₂ D => conjE₂ <| D.weak Δ
+  | disjI₁ D => disjI₁ <| D.weak Δ
+  | disjI₂ D => disjI₂ <| D.weak Δ
+  | @disjE _ _ _ A B _ D D' D'' =>
+    disjE (D.weak Δ)
+      ((Finset.insert_union A Γ Δ) ▸ D'.weak Δ)
+      ((Finset.insert_union B Γ Δ) ▸ D''.weak Δ)
+  | @implI _ _ A B Γ D => implI (Γ ∪ Δ) <| (Finset.insert_union A Γ Δ) ▸ D.weak Δ
+  | implE D D' => implE (D.weak Δ) (D'.weak Δ)
 
-theorem Derivable.tne {A B : Proposition Atom} :
-    Derivable ⟨{((A.impl B).impl B).impl B}, A.impl B⟩ := ⟨Derivation.tne⟩
+def Derivation.weak' {Γ Δ : Ctx Atom} {A : Proposition Atom} (h : Γ ⊆ Δ) (D : Derivation ⟨Γ, A⟩) :
+    Derivation ⟨Δ, A⟩ := Finset.union_sdiff_of_subset h ▸ D.weak (Δ \ Γ)
 
-def tneEquiv {A B : Proposition Atom} :
-    Proposition.equiv (A.impl B) (((A.impl B).impl B).impl B) := ⟨Derivation.dni, Derivation.tne⟩
-
-theorem tne_equivalent {A B : Proposition Atom} :
-    Proposition.Equiv (A.impl B) (((A.impl B).impl B).impl B) := ⟨Derivable.dni, Derivable.tne⟩
-
-/-- Modus tollens -/
-def Derivation.modusTollens {Γ : Ctx Atom} {A B : Proposition Atom} (C : Proposition Atom)
-    (D : Derivation ⟨insert A Γ, B⟩) : Derivation ⟨insert (B.impl C) Γ, A.impl C⟩ :=
-  implI _ <|
-  implE (A := B)
-    (ax' (by grind))
-    (D.weak' (h := by grind))
-
-theorem Derivable.modus_tollens {Γ : Ctx Atom} {A B : Proposition Atom} (C : Proposition Atom)
-    (h : Derivable ⟨insert A Γ, B⟩) : Derivable ⟨insert (B.impl C) Γ, A.impl C⟩ :=
-  let ⟨D⟩ := h; ⟨D.modusTollens C⟩
-
-/-!
-### De Morgan laws
-
-The following are valid in minimal logic, so we use `impl (-) C` over `~(-) := impl (-) bot`.
--/
-
-/-- (A → C) ∧ (B → C) ⊢ (A ∨ B) → C -/
-def disjImpOfConjImps {A B C : Proposition Atom} :
-    Derivation ⟨{conj (impl A C) (impl B C)}, impl (disj A B) C⟩ :=
-  implI _ <|
-  disjE (A := A) (B := B)
-    (ax _ _)
-    (implE (A := A)
-      (conjE₁ (B := B.impl C) (ax' <| by grind))
-      (ax _ _))
-    (implE (A := B)
-      (conjE₂ (A := A.impl C) (ax' (by grind)))
-      (ax _ _))
-
-/-- (A → C) ∧ (B → C) ⊢ (A ∨ B) → C -/
-theorem disj_imp_of_conj_imps {A B C : Proposition Atom} :
-    Derivable ⟨{conj (impl A C) (impl B C)}, impl (disj A B) C⟩ := ⟨disjImpOfConjImps⟩
-
-/-- (A ∨ B) → C ⊢ (A → C) ∧ (B → C) -/
-def conjImpsOfDisjImp {A B C : Proposition Atom} :
-    Derivation ⟨{impl (disj A B) C}, conj (impl A C) (impl B C)⟩ :=
-  conjI
-    (implI {impl (disj A B) C} <|
-      implE (A := A.disj B) (B := C)
-        (ax' (by grind))
-        (disjI₁ (ax _ _)))
-    (implI {impl (disj A B) C} <|
-      implE (A := A.disj B) (B := C)
-        (ax' (by grind))
-        (disjI₂ (ax _ _)))
-
-/-- (A ∨ B) → C ⊢ (A → C) ∧ (B → C) -/
-theorem conj_imps_of_disj_imp {A B C : Proposition Atom} :
-    Derivable ⟨{impl (disj A B) C}, conj (impl A C) (impl B C)⟩ := ⟨conjImpsOfDisjImp⟩
-
-def disjImpConjImpsEquiv {A B C : Proposition Atom} :
-    Proposition.equiv (impl (disj A B) C) (conj (impl A C) (impl B C)) :=
-  ⟨conjImpsOfDisjImp, disjImpOfConjImps⟩
-
-theorem disj_imp_conj_imps_equivalent {A B C : Proposition Atom} :
-    Proposition.Equiv (impl (disj A B) C) (conj (impl A C) (impl B C)) :=
-  ⟨conj_imps_of_disj_imp, disj_imp_of_conj_imps⟩
-
-/-- (A → C) ∨ (B → C) ⊢ (A ∧ B) → C -/
-def conjImpOfDisjImps {A B C : Proposition Atom} :
-    Derivation ⟨{disj (impl A C) (impl B C)}, impl (conj A B) C⟩ := by
-  apply implI
-  apply disjE (A := A.impl C) (B := B.impl C)
-  · exact ax' (by grind)
-  · apply implE (A := A)
-    · apply ax
-    · apply conjE₁ (B := B)
-      exact ax' (by grind)
-  · apply implE (A := B)
-    · apply ax
-    · apply conjE₂ (A := A)
-      exact ax' (by grind)
-
-/-- (A → C) ∨ (B → C) ⊢ (A ∧ B) → C -/
-theorem conj_imp_of_disj_imps {A B C : Proposition Atom} :
-    Derivable ⟨{disj (impl A C) (impl B C)}, impl (conj A B) C⟩ := ⟨conjImpOfDisjImps⟩
-
-/-! ### Further equivalences and implications -/
-
-/-- Equivalence of A → (B → C) and (A ∧ B) → C -/
-def curryEquiv {A B C : Proposition Atom} :
-    Proposition.equiv (A.impl (B.impl C)) (impl (A.conj B) C) := by
+theorem sDerivable_iff {S : Sequent Atom} : SDerivable S ↔ Nonempty (Derivation S) := by
   constructor
-  · apply implI
-    apply implE (A := B)
-    · apply implE (A := A)
-      · exact ax' (by grind)
-      · apply conjE₁ (B := B)
-        exact ax' (by grind)
-    · apply conjE₂ (A := A)
-      exact ax' (by grind)
-  · apply implI
+  · intro ⟨Γ, hΓ, D⟩
+    refine ⟨D.weak' ?_⟩
+    simpa using hΓ
+  · intro ⟨D⟩
+    refine ⟨S.1, by simp, D⟩
+
+theorem Theory.SDerivable.sequent_weak (T : Theory Atom) {Γ Δ : Ctx Atom} {A : Proposition Atom} :
+    T.SDerivable ⟨Γ, A⟩ → T.SDerivable ⟨Γ ∪ Δ, A⟩
+  | .der Γ' hΓ' D => by refine ⟨Γ' ∪ Δ, ?_, D.weak Δ⟩; trans T ∪ Γ ∪ Δ <;> grind
+
+theorem Theory.SDerivable.sequent_weak' (T : Theory Atom) {Γ Δ : Ctx Atom} {A : Proposition Atom}
+    (h_ext : Γ ⊆ Δ) : T.SDerivable ⟨Γ, A⟩ → T.SDerivable ⟨Δ, A⟩
+  | .der Γ' hΓ' D => by refine ⟨Γ' ∪ Δ, ?_, D.weak Δ⟩; trans T ∪ Γ ∪ Δ <;> grind
+
+theorem SDerivable.weak {Γ Δ : Ctx Atom} {A : Proposition Atom} (_ : SDerivable ⟨Γ, A⟩) :
+    SDerivable ⟨Γ ∪ Δ, A⟩ := by
+  apply Theory.SDerivable.sequent_weak; assumption
+
+theorem SDerivable.weak' {Γ Δ : Ctx Atom} {A : Proposition Atom} (h_ext : Γ ⊆ Δ)
+    (_ : SDerivable ⟨Γ, A⟩) : SDerivable ⟨Δ, A⟩ := by
+  apply Theory.SDerivable.sequent_weak' <;> assumption
+
+/-- Substitution of a derivation `E` for one of the hypotheses in the context `Γ` of `D`. -/
+def Derivation.subs {Γ Δ : Ctx Atom} {A B : Proposition Atom}
+    (D : Derivation ⟨Γ, B⟩) (E : Derivation ⟨Δ, A⟩) : Derivation ⟨(Γ \ {A}) ∪ Δ, B⟩ := by
+  match D with
+  | ax _ _ =>
+    by_cases B = A
+    case pos h =>
+      rw [h, Finset.union_comm]
+      exact E.weak _
+    case neg h =>
+      rw [Finset.insert_sdiff_of_notMem (h := Finset.notMem_singleton.mpr h)]
+      exact (ax _ B).weak _
+  | botE _ D => exact botE B <| D.subs E
+  | conjI D D' => exact conjI (D.subs E) (D'.subs E)
+  | conjE₁ D => exact conjE₁ <| D.subs E
+  | conjE₂ D => exact conjE₂ <| D.subs E
+  | disjI₁ D => exact disjI₁ <| D.subs E
+  | disjI₂ D => exact disjI₂ <| D.subs E
+  | @disjE _ _ _ C C' B D D' D'' =>
+    apply disjE (D.subs E)
+    · by_cases C = A
+      case pos h =>
+        rw [h] at D' ⊢
+        have : insert A ((Γ \ {A}) ∪ Δ) = (insert A Γ) ∪ Δ := by grind
+        rw [this]
+        exact D'.weak _
+      case neg h =>
+        have : insert C ((Γ \ {A}) ∪ Δ) = ((insert C Γ) \ {A}) ∪ Δ := by grind
+        rw [this]
+        exact D'.subs E
+    · by_cases C' = A
+      case pos h =>
+        rw [h] at D'' ⊢
+        have : insert A ((Γ \ {A}) ∪ Δ) = (insert A Γ) ∪ Δ := by grind
+        rw [this]
+        exact D''.weak _
+      case neg h =>
+        have : insert C' ((Γ \ {A}) ∪ Δ) = ((insert C' Γ) \ {A}) ∪ Δ := by grind
+        rw [this]
+        exact D''.subs E
+  | @implI _ _ A' B _ D =>
     apply implI
-    apply implE (A := A.conj B)
-    · exact ax' (by grind)
-    · apply conjI <;> exact ax' (by grind)
+    by_cases A' = A
+    case pos h =>
+      rw [h] at D ⊢
+      have : insert A (Γ \ {A} ∪ Δ) = insert A Γ ∪ Δ := by grind
+      rw [this]
+      exact D.weak Δ
+    case neg h =>
+      have : insert A' ((Γ \ {A}) ∪ Δ) = ((insert A' Γ) \ {A}) ∪ Δ := by grind
+      rw [this]
+      exact D.subs E
+  | implE D D' => exact implE (D.subs E) (D'.subs E)
 
-/-- Equivalence of A → (B → C) and (A ∧ B) → C -/
-theorem curry_equiv {A B C : Proposition Atom} :
-    Proposition.Equiv (A.impl (B.impl C)) (impl (A.conj B) C) := ⟨⟨curryEquiv.1⟩, ⟨curryEquiv.2⟩⟩
+theorem Theory.SDerivable.subs {T : Theory Atom} {Γ Δ : Ctx Atom} {A B : Proposition Atom} :
+    T.SDerivable ⟨Γ, B⟩ → T.SDerivable ⟨Δ, A⟩ → T.SDerivable ⟨(Γ \ {A}) ∪ Δ, B⟩
+  | .der Γ' hΓ' D, .der Δ' hΔ' E =>
+    ⟨Γ' \ {A} ∪ Δ', by grind [Finset.coe_union, Finset.coe_sdiff], D.subs E⟩
 
-/-- A ∧ B ⊢ B ∧ A -/
-def conjCommDer {A B : Proposition Atom} : Derivation ⟨{A.conj B}, B.conj A⟩ := by
-  apply conjI
-  · apply conjE₂ (A := A)
-    exact ax' (by grind)
-  · apply conjE₁ (B := B)
-    exact ax' (by grind)
+def Derivation.subs' {Γ : Ctx Atom} {A B : Proposition Atom}
+    (D : Derivation ⟨{A}, B⟩) (E : Derivation ⟨Γ, A⟩) : Derivation ⟨Γ, B⟩ := by
+  have : Γ = ({A} \ {A}) ∪ Γ := by grind
+  rw [this]
+  exact D.subs E
 
-/-- Equivalence of A ∧ B and B ∧ A -/
-def conjCommEquiv {A B : Proposition Atom} : Proposition.equiv (A.conj B) (B.conj A) :=
-  ⟨conjCommDer, conjCommDer⟩
-
-/-- Equivalence of A ∧ B and B ∧ A -/
-theorem conj_comm_equiv {A B : Proposition Atom} : Proposition.Equiv (A.conj B) (B.conj A) :=
-  ⟨⟨conjCommDer⟩, ⟨conjCommDer⟩⟩
-
-/-- Equivalence of A ∧ A and A -/
-def conjIdemEquiv {A : Proposition Atom} : Proposition.equiv (A.conj A) A := by
-  constructor
-  · apply conjE₁ (B := A)
-    exact ax' (by grind)
-  · apply conjI <;> exact ax' (by grind)
-
-/-- Equivalence of A ∧ A and A -/
-theorem conj_idem_equiv {A : Proposition Atom} : Proposition.Equiv (A.conj A) A :=
-  ⟨⟨conjIdemEquiv.1⟩, ⟨conjIdemEquiv.2⟩⟩
-
-/-- A ∨ B ⊢ B ∨ A -/
-def disjCommDer {A B : Proposition Atom} : Derivation ⟨{A.disj B}, B.disj A⟩ := by
-  apply disjE (A := A) (B := B)
-  · exact ax' (by grind)
-  · apply disjI₂
-    exact ax' (by grind)
-  · apply disjI₁
-    exact ax' (by grind)
-
-/-- Equivalence of A ∨ B and B ∨ A -/
-def disjCommEquiv {A B : Proposition Atom} : Proposition.equiv (A.disj B) (B.disj A) :=
-  ⟨disjCommDer, disjCommDer⟩
-
-/-- Equivalence of A ∨ B and B ∨ A -/
-theorem disj_comm_equiv {A B : Proposition Atom} : Proposition.Equiv (A.disj B) (B.disj A) :=
-  ⟨⟨disjCommDer⟩, ⟨disjCommDer⟩⟩
-
-/-- Equivalence of A ∨ A and A -/
-def disjIdemEquiv {A : Proposition Atom} : Proposition.equiv (A.disj A) A := by
-  constructor
-  · apply disjE (A := A) (B := A) <;> exact ax' (by grind)
-  · apply disjI₁
-    exact ax' (by grind)
-
-/-- Equivalence of A ∨ A and A -/
-theorem disj_idem_equiv {A : Proposition Atom} : Proposition.Equiv (A.disj A) A :=
-  ⟨⟨disjIdemEquiv.1⟩, ⟨disjIdemEquiv.2⟩⟩
-
-/-- Equivalence of A → (A → B) and A → B -/
-def implIdemEquiv {A B : Proposition Atom} :
-    Proposition.equiv (A.impl <| A.impl B) (A.impl B) := by
-  constructor
-  · apply implI
+theorem Theory.SDerivable.subs' {T : Theory Atom} {Γ : Ctx Atom} {A B : Proposition Atom} :
+    T.Derivable (A.impl B) → T.SDerivable ⟨Γ, A⟩ → T.SDerivable ⟨Γ, B⟩
+  | ⟨Δ, hΔ, E⟩, ⟨Γ', hΓ', D⟩ => by
+    refine ⟨Δ ∪ Γ', by grind, ?_⟩
     apply implE (A := A)
-    · apply implE (A := A)
-      · exact ax' (by grind)
-      · exact ax' (by grind)
-    · exact ax' (by grind)
-  · apply implI
-    exact ax' (by grind)
+    · exact E.weak' (by grind)
+    · exact D.weak' (by grind)
 
-/-- Equivalence of A → (A → B) and A → B -/
-theorem impl_idem_equiv {A B : Proposition Atom} :
-    Proposition.Equiv (A.impl <| A.impl B) (A.impl B) := ⟨⟨implIdemEquiv.1⟩, ⟨implIdemEquiv.2⟩⟩
+theorem SDerivable.subs {Γ Δ : Ctx Atom} {A B : Proposition Atom} :
+    SDerivable ⟨Γ, B⟩ → SDerivable ⟨Δ, A⟩ → SDerivable ⟨(Γ \ {A}) ∪ Δ, B⟩ := Theory.SDerivable.subs
 
-/-- A → (B → C) ⊢ B → (A → C) -/
-def implSwapDer {A B C : Proposition Atom} :
-    Derivation ⟨{A.impl <| B.impl C}, B.impl (A.impl C)⟩ := by
-  apply implI
-  apply implI
-  apply implE (A := B)
-  · apply implE (A := A) <;> exact ax' (by grind)
-  · exact ax' (by grind)
+theorem SDerivable.subs' {Γ : Ctx Atom} {A B : Proposition Atom} :
+    (h : Derivable (A.impl B)) → (h' : SDerivable ⟨Γ, A⟩) → SDerivable ⟨Γ, B⟩ :=
+  Theory.SDerivable.subs'
 
-/-- Equivalence of A → (B → C) and B → (A → C) -/
-def implSwapEquiv {A B C : Proposition Atom} :
-    Proposition.equiv (A.impl <| B.impl C) (B.impl (A.impl C)) := ⟨implSwapDer, implSwapDer⟩
+/-! ### Inference rules for derivability -/
 
-/-- A → (B → C) ⊢ (A → B) → (A → C) -/
-def implImplDistrib {A B C : Proposition Atom} :
-    Derivation ⟨{A.impl (B.impl C)}, impl (A.impl B) (A.impl C)⟩ := by
-  apply implI
-  apply implI
-  apply implE (A := B) <;> apply implE (A := A) <;> exact ax' (by grind)
+theorem Theory.Derivable.ax' {T : Theory Atom} {A : Proposition Atom} (h : A ∈ T) :
+  T.Derivable A := ⟨{A}, by grind, Derivation.ax ∅ A⟩
 
-theorem impl_impl_distrib {A B C : Proposition Atom} :
-    Derivable ⟨{A.impl (B.impl C)}, impl (A.impl B) (A.impl C)⟩ := ⟨implImplDistrib⟩
+theorem Theory.Derivable.botE {T : Theory Atom} (A : Proposition Atom) :
+    T.Derivable Proposition.bot → T.Derivable A
+  | ⟨Γ, h, D⟩ => ⟨Γ, h, Derivation.botE A D⟩
 
-/-- Equivalence of A → (B → C) and B → (A → C) -/
-theorem impl_swap_equiv {A B C : Proposition Atom} :
-    Proposition.Equiv (A.impl <| B.impl C) (B.impl (A.impl C)) := ⟨⟨implSwapDer⟩, ⟨implSwapDer⟩⟩
+theorem Theory.Derivable.conjI {T : Theory Atom} {A B : Proposition Atom} :
+    T.Derivable A → T.Derivable B → T.Derivable (A.conj B)
+  | ⟨Γ, h, D⟩, ⟨Γ', h', D'⟩ =>
+    ⟨Γ ∪ Γ', by grind, Derivation.conjI (D.weak' (by grind)) (D'.weak' (by grind))⟩
 
-/-- Equivalence of A ∧ (A ∨ B) and A -/
-def absorbConjDisj {A B : Proposition Atom} : Proposition.equiv (A.conj <| (A.disj B)) A := by
+theorem Theory.Derivable.conjE₁ {T : Theory Atom} {A B : Proposition Atom} :
+    T.Derivable (A.conj B) → T.Derivable A
+  | ⟨Γ, h, D⟩ => ⟨Γ, h, D.conjE₁⟩
+
+theorem Theory.Derivable.conjE₂ {T : Theory Atom} {A B : Proposition Atom} :
+    T.Derivable (A.conj B) → T.Derivable B
+  | ⟨Γ, h, D⟩ => ⟨Γ, h, D.conjE₂⟩
+
+theorem Theory.Derivable.disjI₁ {T : Theory Atom} {A B : Proposition Atom} :
+    T.Derivable A → T.Derivable (A.disj B)
+  | ⟨Γ, h, D⟩ => ⟨Γ, h, D.disjI₁⟩
+
+theorem Theory.Derivable.disjI₂ {T : Theory Atom} {A B : Proposition Atom} :
+    T.Derivable B → T.Derivable (A.disj B)
+  | ⟨Γ, h, D⟩ => ⟨Γ, h, D.disjI₂⟩
+
+theorem Theory.Derivable.disjE {T : Theory Atom} {A B C : Proposition Atom} :
+    T.Derivable (A.disj B) → T.Derivable (A.impl C) → T.Derivable (B.impl C) → T.Derivable C
+  | ⟨Γ, h, D⟩, ⟨Δ₁, h₁, E₁⟩, ⟨Δ₂, h₂, E₂⟩ => by
+    refine ⟨Γ ∪ Δ₁ ∪ Δ₂, by grind, ?_⟩
+    apply Derivation.disjE (A := A) (B := B)
+    · exact D.weak' (by grind)
+    · apply Derivation.implE (A := A)
+      · exact E₁.weak' (by grind)
+      · exact Derivation.ax' (by grind)
+    · apply Derivation.implE (A := B)
+      · exact E₂.weak' (by grind)
+      · exact Derivation.ax' (by grind)
+
+theorem Theory.Derivable.implE {T : Theory Atom} {A B : Proposition Atom} :
+    T.Derivable (A.impl B) → T.Derivable A → T.Derivable B
+  | ⟨Γ₁, h₁, D₁⟩, ⟨Γ₂, h₂, D₂⟩ => by
+    refine ⟨Γ₁ ∪ Γ₂, by grind, ?_⟩
+    exact Derivation.implE (A := A) (D₁.weak' (by grind)) (D₂.weak' (by grind))
+
+theorem Theory.Derivable.trans {T : Theory Atom} {A B C : Proposition Atom} :
+    T.Derivable (A.impl B) → T.Derivable (B.impl C) → T.Derivable (A.impl C)
+  | ⟨Γ₁, h₁, D₁⟩, ⟨Γ₂, h₂, D₂⟩ => by
+    refine ⟨Γ₁ ∪ Γ₂, by grind, ?_⟩
+    apply implI
+    apply Derivation.implE (A := B)
+    · exact D₂.weak' (by grind)
+    · apply Derivation.implE (A := A)
+      · exact D₁.weak' (by grind)
+      · exact Derivation.ax' (by grind)
+
+/-! ### Properties of NJ-equivalence -/
+
+theorem equiv_iff {A B : Proposition Atom} : Equiv A B ↔ Nonempty (Proposition.equiv A B) := by
   constructor
-  · apply conjE₁ (B := (A.disj B))
-    exact ax' (by grind)
-  · apply conjI
+  · intro ⟨hAB, hBA⟩
+    let ⟨DAB⟩ := derivable_iff.mp hAB
+    let ⟨DBA⟩ := derivable_iff.mp hBA
+    refine ⟨?_,?_⟩
+    · refine Derivation.implE (DAB.weak' (by grind)) (ax' <| by grind)
+    · refine Derivation.implE (DBA.weak' (by grind)) (ax' <| by grind)
+  · intro ⟨DAB, DBA⟩
+    refine ⟨?_,?_⟩
+    all_goals apply derivable_iff.mpr; constructor; apply implI; assumption
+
+
+theorem Proposition.derivable_iff_equiv_top (T : Theory Atom) (A : Proposition Atom) :
+    T.Derivable A ↔ T.Equiv A top := by
+  constructor <;> intro h
+  · constructor
+    · refine ⟨∅, by grind, ?_⟩
+      exact implI (A := A) (B := Proposition.top) ∅ <| derivationTop.weak' (by grind)
+    · let ⟨Γ, hΓ, D⟩ := h
+      refine ⟨Γ, by grind, ?_⟩
+      refine implI Γ <| D.weak' (by grind)
+  · let ⟨Γ, hΓ, D⟩ := h.2
+    refine ⟨Γ, by grind, ?_⟩
+    exact implE (A := Proposition.top) D <| derivationTop.weak' (by grind)
+
+/-- Change the conclusion along an equivalence. -/
+def mapEquivConclusion (Γ : Ctx Atom) {A B : Proposition Atom} (e : Proposition.equiv A B) :
+    Derivation ⟨Γ, A⟩ → Derivation ⟨Γ, B⟩ := e.1.subs'
+
+theorem Theory.equivalent_sDerivable_conclusion {T : Theory Atom} (Γ : Ctx Atom)
+    {A B : Proposition Atom} (h : T.Equiv A B) : T.SDerivable ⟨Γ, A⟩ ↔ T.SDerivable ⟨Γ, B⟩ := by
+  let ⟨⟨Γ₁, hΓ₁, D₁⟩, ⟨Γ₂, hΓ₂, D₂⟩⟩ := h
+  constructor <;> intro ⟨Γ', hΓ, D⟩
+  · refine ⟨Γ₁ ∪ Γ', by grind, ?_⟩
+    apply implE (A := A)
+    · exact D₁.weak' (by grind)
+    · exact D.weak' (by grind)
+  · refine ⟨Γ₂ ∪ Γ', by grind, ?_⟩
+    apply implE (A := B)
+    · exact D₂.weak' (by grind)
+    · exact D.weak' (by grind)
+
+theorem equivalent_sDerivable_conclusion (Γ : Ctx Atom) {A B : Proposition Atom} (h : Equiv A B) :
+    SDerivable ⟨Γ, A⟩ ↔ SDerivable ⟨Γ, B⟩ :=
+  (Theory.empty Atom).equivalent_sDerivable_conclusion Γ h
+
+/-- Replace a hypothesis along an equivalence. -/
+def mapEquivHypothesis (Γ : Ctx Atom) {A B : Proposition Atom} (e : Proposition.equiv A B)
+    (C : Proposition Atom) (D : Derivation ⟨insert A Γ, C⟩) : Derivation ⟨insert B Γ, C⟩ := by
+  have : insert B Γ = (insert A Γ \ {A}) ∪ (insert B Γ) := by grind
+  rw [this]
+  refine D.subs ?_
+  exact e.2.weak' (by grind)
+
+theorem equivalent_hypotheses {T : Theory Atom} (Γ : Ctx Atom) {A B : Proposition Atom}
+    (h : T.Equiv A B) (C : Proposition Atom) :
+    T.SDerivable ⟨insert A Γ, C⟩ ↔ T.SDerivable ⟨insert B Γ, C⟩ := by
+  let ⟨⟨Γ₁, hΓ₁, D₁⟩, ⟨Γ₂, hΓ₂, D₂⟩⟩ := h
+  constructor <;> intro h'
+  · have : insert B Γ = (insert A Γ \ {A}) ∪ (insert B Γ) := by grind
+    rw [this]
+    apply Theory.SDerivable.subs h'
+    refine ⟨insert B Γ₁ ∪ Γ₂, by grind, ?_⟩
+    apply implE (A := B)
+    · exact D₂.weak' (by grind)
     · exact ax' (by grind)
-    · apply disjI₁
-      exact ax' (by grind)
-
-/-- Equivalence of A ∧ (A ∨ B) and A -/
-theorem absorb_conj_disj {A B : Proposition Atom} : Proposition.Equiv (A.conj <| (A.disj B)) A :=
-  ⟨⟨absorbConjDisj.1⟩, ⟨absorbConjDisj.2⟩⟩
-
-/-- Equivalence of A ∨ (A ∧ B) and A -/
-def absorbDisjConj {A B : Proposition Atom} : Proposition.equiv (A.disj <| A.conj B) A := by
-  constructor
-  · apply disjE (A := A) (B := A.conj B)
-    · exact ax' (by grind)
-    · exact ax' (by grind)
-    · apply conjE₁ (B := B)
-      exact ax' (by grind)
-  · apply disjI₁
-    exact ax' (by grind)
-
-/-- Equivalence of A ∨ (A ∧ B) and A -/
-theorem absorb_disj_conj {A B : Proposition Atom} :  Proposition.Equiv (A.disj <| A.conj B) A :=
-  ⟨⟨absorbDisjConj.1⟩, ⟨absorbDisjConj.2⟩⟩
-
-/-- Falsum is absorbing for conjunction -/
-def botConjAbsorb {A : Proposition Atom} : Proposition.equiv (A.conj bot) bot := by
-  constructor
-  · apply conjE₂ (A := A)
-    exact ax' (by grind)
-  · apply conjI
-    · apply botE
-      exact ax' (by grind)
+  · have : insert A Γ = (insert B Γ \ {B}) ∪ (insert A Γ) := by grind
+    rw [this]
+    apply Theory.SDerivable.subs h'
+    refine ⟨insert A Γ₂ ∪ Γ₁, by grind, ?_⟩
+    apply implE (A := A)
+    · exact D₁.weak' (by grind)
     · exact ax' (by grind)
 
-/-- Falsum is absorbing for conjunction -/
-theorem bot_conj_absorb {A : Proposition Atom} : Proposition.Equiv (A.conj bot) bot :=
-  ⟨⟨botConjAbsorb.1⟩, ⟨botConjAbsorb.2⟩⟩
+def reflEquiv (A : Proposition Atom) : Proposition.equiv A A :=
+  let D : Derivation ⟨{A},A⟩ := ax' <| by grind;
+  ⟨D,D⟩
 
-/-- Falsum is neutral for disjunction -/
-def botDisjNeutral {A : Proposition Atom} : Proposition.equiv (A.disj bot) A := by
-  constructor
-  · apply disjE (A := A) (B := bot)
-    · exact ax' (by grind)
-    · exact ax' (by grind)
-    · apply botE
-      exact ax' (by grind)
-  · apply disjI₁
-    exact ax' (by grind)
+def commEquiv {A B : Proposition Atom} (e : Proposition.equiv A B) : Proposition.equiv B A :=
+  ⟨e.2, e.1⟩
 
-/-- Falsum is neutral for disjunction -/
-theorem bot_disj_neutral {A : Proposition Atom} : Proposition.Equiv (A.disj bot) A :=
-  ⟨⟨botDisjNeutral.1⟩, ⟨botDisjNeutral.2⟩⟩
+def transEquiv {A B C : Proposition Atom} (eAB : Proposition.equiv A B)
+    (eBC : Proposition.equiv B C) : Proposition.equiv A C :=
+  ⟨mapEquivConclusion _ eBC eAB.1, mapEquivConclusion _ (commEquiv eAB) eBC.2⟩
+
+theorem equivalent_refl {T : Theory Atom} (A : Proposition Atom) : T.Equiv A A := by
+  have : T.Derivable (A.impl A) := by refine ⟨∅, by grind, ?_⟩; apply implI; exact ax' (by grind)
+  grind [Theory.Equiv]
+
+theorem equivalent_comm {T : Theory Atom} {A B : Proposition Atom} :
+    T.Equiv A B → T.Equiv B A := by grind [Theory.Equiv]
+
+theorem equivalent_trans {T : Theory Atom} {A B C : Proposition Atom} :
+    T.Equiv A B → T.Equiv B C → T.Equiv A C
+  | ⟨AB, BA⟩, ⟨BC, CB⟩ => ⟨AB.trans BC, CB.trans BA⟩
+
+/-- Equivalence is indeed an equivalence relation. -/
+theorem Theory.equiv_equivalence (T : Theory Atom) : Equivalence (T.Equiv (Atom := Atom)) :=
+  ⟨equivalent_refl, equivalent_comm, equivalent_trans⟩
+
+protected def Theory.propositionSetoid (T : Theory Atom) : Setoid (Proposition Atom) :=
+  ⟨T.Equiv, T.equiv_equivalence⟩
 
 end NJ
 
