Cslib/Logics/IPL/NJ/Theorems.lean
@@ -1,0 +1,331 @@
+/-
+Copyright (c) 2025 Thomas Waring. All rights reserved.
+Released under Apache 2.0 license as described in the file LICENSE.
+Authors: Thomas Waring
+-/
+import Cslib.Logics.IPL.NJ.Basic
+
+/-! # Elementary derivations and equivalences in NJ -/
+
+variable {Atom : Type u} [DecidableEq Atom]
+
+namespace IPL
+
+open Proposition
+
+namespace NJ
+
+open Derivation
+
+/-!
+### Negation theorems
+
+The following are valid in minimal logic, so we use `impl (-) C` over `~(-) := impl (-) bot`.
+-/
+
+/-- Double negation introduction -/
+def Derivation.dni {A B : Proposition Atom} : Derivation ⟨{A}, impl (impl A B) B⟩ :=
+  implI (A := A.impl B) _ <|
+  implE (A := A) (ax' (by grind)) (ax' (by grind))
+
+theorem SDerivable.dni {A B : Proposition Atom} : SDerivable ⟨{A},impl (impl A B) B⟩ :=
+  sDerivable_iff.mpr ⟨Derivation.dni⟩
+
+/-- The double negation of excluded-middle, or in minimal-logic-style ⊢ (A ∨ (A → B)) → B → B. -/
+def Derivation.notNotLEM {A B : Proposition Atom} :
+    Derivation ⟨∅, (A.disj <| impl A B).impl B |>.impl B⟩ :=
+  implI _ <|
+  implE (A := A.disj (A.impl B)) (ax' <| by grind) <|
+  disjI₂ <|
+  implI _ <|
+  implE (A := A.disj (A.impl B)) (ax' <| by grind) <|
+  disjI₁ <|
+  ax' <| by grind
+
+theorem Derivable.not_not_lem {A B : Proposition Atom} :
+    SDerivable ⟨∅, (A.disj <| impl A B).impl B |>.impl B⟩ :=
+  sDerivable_iff.mpr ⟨Derivation.notNotLEM⟩
+
+/-- Triple negation elimination -/
+def Derivation.tne {A B : Proposition Atom} :
+    Derivation ⟨{((A.impl B).impl B).impl B}, A.impl B⟩ :=
+  implI _ <|
+  implE (A := (A.impl B).impl B) (ax' <| by grind) <|
+  Derivation.dni.weak' (Γ := {A}) (by grind)
+
+theorem Derivable.tne {A B : Proposition Atom} :
+    SDerivable ⟨{((A.impl B).impl B).impl B}, A.impl B⟩ := sDerivable_iff.mpr ⟨Derivation.tne⟩
+
+def tneEquiv {A B : Proposition Atom} :
+    Proposition.equiv (A.impl B) (((A.impl B).impl B).impl B) := ⟨Derivation.dni, Derivation.tne⟩
+
+theorem tne_equivalent {A B : Proposition Atom} :
+    Equiv (A.impl B) (((A.impl B).impl B).impl B) := equiv_iff.mpr ⟨tneEquiv⟩
+
+/-- Modus tollens -/
+def Derivation.modusTollens {Γ : Ctx Atom} {A B : Proposition Atom} (C : Proposition Atom)
+    (D : Derivation ⟨insert A Γ, B⟩) : Derivation ⟨insert (B.impl C) Γ, A.impl C⟩ :=
+  implI _ <|
+  implE (A := B)
+    (ax' (by grind))
+    (D.weak' (h := by grind))
+
+theorem Derivable.modus_tollens {Γ : Ctx Atom} {A B : Proposition Atom} (C : Proposition Atom)
+    (h : SDerivable ⟨insert A Γ, B⟩) : SDerivable ⟨insert (B.impl C) Γ, A.impl C⟩ :=
+  let ⟨D⟩ := sDerivable_iff.mp h; sDerivable_iff.mpr ⟨D.modusTollens C⟩
+
+/-!
+### De Morgan laws
+
+The following are valid in minimal logic, so we use `impl (-) C` over `~(-) := impl (-) bot`.
+-/
+
+/-- (A → C) ∧ (B → C) ⊢ (A ∨ B) → C -/
+def disjImpOfConjImps {A B C : Proposition Atom} :
+    Derivation ⟨{conj (impl A C) (impl B C)}, impl (disj A B) C⟩ :=
+  implI _ <|
+  disjE (A := A) (B := B)
+    (ax _ _)
+    (implE (A := A)
+      (conjE₁ (B := B.impl C) (ax' <| by grind))
+      (ax _ _))
+    (implE (A := B)
+      (conjE₂ (A := A.impl C) (ax' (by grind)))
+      (ax _ _))
+
+/-- (A → C) ∧ (B → C) ⊢ (A ∨ B) → C -/
+theorem disj_imp_of_conj_imps {A B C : Proposition Atom} :
+    SDerivable ⟨{conj (impl A C) (impl B C)}, impl (disj A B) C⟩ :=
+  sDerivable_iff.mpr ⟨disjImpOfConjImps⟩
+
+/-- (A ∨ B) → C ⊢ (A → C) ∧ (B → C) -/
+def conjImpsOfDisjImp {A B C : Proposition Atom} :
+    Derivation ⟨{impl (disj A B) C}, conj (impl A C) (impl B C)⟩ :=
+  conjI
+    (implI {impl (disj A B) C} <|
+      implE (A := A.disj B) (B := C)
+        (ax' (by grind))
+        (disjI₁ (ax _ _)))
+    (implI {impl (disj A B) C} <|
+      implE (A := A.disj B) (B := C)
+        (ax' (by grind))
+        (disjI₂ (ax _ _)))
+
+/-- (A ∨ B) → C ⊢ (A → C) ∧ (B → C) -/
+theorem conj_imps_of_disj_imp {A B C : Proposition Atom} :
+    SDerivable ⟨{impl (disj A B) C}, conj (impl A C) (impl B C)⟩ :=
+  sDerivable_iff.mpr ⟨conjImpsOfDisjImp⟩
+
+def disjImpConjImpsEquiv {A B C : Proposition Atom} :
+    Proposition.equiv (impl (disj A B) C) (conj (impl A C) (impl B C)) :=
+  ⟨conjImpsOfDisjImp, disjImpOfConjImps⟩
+
+theorem disj_imp_conj_imps_equivalent {A B C : Proposition Atom} :
+    Equiv (impl (disj A B) C) (conj (impl A C) (impl B C)) :=
+  equiv_iff.mpr ⟨disjImpConjImpsEquiv⟩
+
+/-- (A → C) ∨ (B → C) ⊢ (A ∧ B) → C -/
+def conjImpOfDisjImps {A B C : Proposition Atom} :
+    Derivation ⟨{disj (impl A C) (impl B C)}, impl (conj A B) C⟩ := by
+  apply implI
+  apply disjE (A := A.impl C) (B := B.impl C)
+  · exact ax' (by grind)
+  · apply implE (A := A)
+    · apply ax
+    · apply conjE₁ (B := B)
+      exact ax' (by grind)
+  · apply implE (A := B)
+    · apply ax
+    · apply conjE₂ (A := A)
+      exact ax' (by grind)
+
+/-- (A → C) ∨ (B → C) ⊢ (A ∧ B) → C -/
+theorem conj_imp_of_disj_imps {A B C : Proposition Atom} :
+    SDerivable ⟨{disj (impl A C) (impl B C)}, impl (conj A B) C⟩ :=
+  sDerivable_iff.mpr ⟨conjImpOfDisjImps⟩
+
+/-! ### Further equivalences and implications -/
+
+/-- Equivalence of A → (B → C) and (A ∧ B) → C -/
+def curryEquiv {A B C : Proposition Atom} :
+    Proposition.equiv (A.impl (B.impl C)) (impl (A.conj B) C) := by
+  constructor
+  · apply implI
+    apply implE (A := B)
+    · apply implE (A := A)
+      · exact ax' (by grind)
+      · apply conjE₁ (B := B)
+        exact ax' (by grind)
+    · apply conjE₂ (A := A)
+      exact ax' (by grind)
+  · apply implI
+    apply implI
+    apply implE (A := A.conj B)
+    · exact ax' (by grind)
+    · apply conjI <;> exact ax' (by grind)
+
+/-- Equivalence of A → (B → C) and (A ∧ B) → C -/
+theorem curry_equiv {A B C : Proposition Atom} :
+    Equiv (A.impl (B.impl C)) (impl (A.conj B) C) := equiv_iff.mpr ⟨curryEquiv⟩
+
+/-- A ∧ B ⊢ B ∧ A -/
+def conjCommDer {A B : Proposition Atom} : Derivation ⟨{A.conj B}, B.conj A⟩ := by
+  apply conjI
+  · apply conjE₂ (A := A)
+    exact ax' (by grind)
+  · apply conjE₁ (B := B)
+    exact ax' (by grind)
+
+/-- Equivalence of A ∧ B and B ∧ A -/
+def conjCommEquiv {A B : Proposition Atom} : Proposition.equiv (A.conj B) (B.conj A) :=
+  ⟨conjCommDer, conjCommDer⟩
+
+/-- Equivalence of A ∧ B and B ∧ A -/
+theorem conj_comm_equiv {A B : Proposition Atom} : Equiv (A.conj B) (B.conj A) :=
+  equiv_iff.mpr ⟨conjCommEquiv⟩
+
+/-- Equivalence of A ∧ A and A -/
+def conjIdemEquiv {A : Proposition Atom} : Proposition.equiv (A.conj A) A := by
+  constructor
+  · apply conjE₁ (B := A)
+    exact ax' (by grind)
+  · apply conjI <;> exact ax' (by grind)
+
+/-- Equivalence of A ∧ A and A -/
+theorem conj_idem_equiv {A : Proposition Atom} : Equiv (A.conj A) A :=
+  equiv_iff.mpr ⟨conjIdemEquiv⟩
+
+/-- A ∨ B ⊢ B ∨ A -/
+def disjCommDer {A B : Proposition Atom} : Derivation ⟨{A.disj B}, B.disj A⟩ := by
+  apply disjE (A := A) (B := B)
+  · exact ax' (by grind)
+  · apply disjI₂
+    exact ax' (by grind)
+  · apply disjI₁
+    exact ax' (by grind)
+
+/-- Equivalence of A ∨ B and B ∨ A -/
+def disjCommEquiv {A B : Proposition Atom} : Proposition.equiv (A.disj B) (B.disj A) :=
+  ⟨disjCommDer, disjCommDer⟩
+
+/-- Equivalence of A ∨ B and B ∨ A -/
+theorem disj_comm_equiv {A B : Proposition Atom} : Equiv (A.disj B) (B.disj A) :=
+  equiv_iff.mpr ⟨disjCommEquiv⟩
+
+/-- Equivalence of A ∨ A and A -/
+def disjIdemEquiv {A : Proposition Atom} : Proposition.equiv (A.disj A) A := by
+  constructor
+  · apply disjE (A := A) (B := A) <;> exact ax' (by grind)
+  · apply disjI₁
+    exact ax' (by grind)
+
+/-- Equivalence of A ∨ A and A -/
+theorem disj_idem_equiv {A : Proposition Atom} : Equiv (A.disj A) A :=
+  equiv_iff.mpr ⟨disjIdemEquiv⟩
+
+/-- Equivalence of A → (A → B) and A → B -/
+def implIdemEquiv {A B : Proposition Atom} :
+    Proposition.equiv (A.impl <| A.impl B) (A.impl B) := by
+  constructor
+  · apply implI
+    apply implE (A := A)
+    · apply implE (A := A)
+      · exact ax' (by grind)
+      · exact ax' (by grind)
+    · exact ax' (by grind)
+  · apply implI
+    exact ax' (by grind)
+
+/-- Equivalence of A → (A → B) and A → B -/
+theorem impl_idem_equiv {A B : Proposition Atom} :
+    Equiv (A.impl <| A.impl B) (A.impl B) := equiv_iff.mpr ⟨implIdemEquiv⟩
+
+/-- A → (B → C) ⊢ B → (A → C) -/
+def implSwapDer {A B C : Proposition Atom} :
+    Derivation ⟨{A.impl <| B.impl C}, B.impl (A.impl C)⟩ := by
+  apply implI
+  apply implI
+  apply implE (A := B)
+  · apply implE (A := A) <;> exact ax' (by grind)
+  · exact ax' (by grind)
+
+/-- Equivalence of A → (B → C) and B → (A → C) -/
+def implSwapEquiv {A B C : Proposition Atom} :
+    Proposition.equiv (A.impl <| B.impl C) (B.impl (A.impl C)) := ⟨implSwapDer, implSwapDer⟩
+
+/-- Equivalence of A → (B → C) and B → (A → C) -/
+theorem impl_swap_equiv {A B C : Proposition Atom} :
+    Equiv (A.impl <| B.impl C) (B.impl (A.impl C)) := equiv_iff.mpr ⟨implSwapEquiv⟩
+
+/-- A → (B → C) ⊢ (A → B) → (A → C) -/
+def implImplDistrib {A B C : Proposition Atom} :
+    Derivation ⟨{A.impl (B.impl C)}, impl (A.impl B) (A.impl C)⟩ := by
+  apply implI
+  apply implI
+  apply implE (A := B) <;> apply implE (A := A) <;> exact ax' (by grind)
+
+theorem impl_impl_distrib {A B C : Proposition Atom} :
+    SDerivable ⟨{A.impl (B.impl C)}, impl (A.impl B) (A.impl C)⟩ :=
+  sDerivable_iff.mpr ⟨implImplDistrib⟩
+
+/-- Equivalence of A ∧ (A ∨ B) and A -/
+def absorbConjDisj {A B : Proposition Atom} : Proposition.equiv (A.conj <| (A.disj B)) A := by
+  constructor
+  · apply conjE₁ (B := (A.disj B))
+    exact ax' (by grind)
+  · apply conjI
+    · exact ax' (by grind)
+    · apply disjI₁
+      exact ax' (by grind)
+
+/-- Equivalence of A ∧ (A ∨ B) and A -/
+theorem absorb_conj_disj {A B : Proposition Atom} : Equiv (A.conj <| (A.disj B)) A :=
+  equiv_iff.mpr ⟨absorbConjDisj⟩
+
+/-- Equivalence of A ∨ (A ∧ B) and A -/
+def absorbDisjConj {A B : Proposition Atom} : Proposition.equiv (A.disj <| A.conj B) A := by
+  constructor
+  · apply disjE (A := A) (B := A.conj B)
+    · exact ax' (by grind)
+    · exact ax' (by grind)
+    · apply conjE₁ (B := B)
+      exact ax' (by grind)
+  · apply disjI₁
+    exact ax' (by grind)
+
+/-- Equivalence of A ∨ (A ∧ B) and A -/
+theorem absorb_disj_conj {A B : Proposition Atom} :  Equiv (A.disj <| A.conj B) A :=
+  equiv_iff.mpr ⟨absorbDisjConj⟩
+
+/-- Falsum is absorbing for conjunction -/
+def botConjAbsorb {A : Proposition Atom} : Proposition.equiv (A.conj bot) bot := by
+  constructor
+  · apply conjE₂ (A := A)
+    exact ax' (by grind)
+  · apply conjI
+    · apply botE
+      exact ax' (by grind)
+    · exact ax' (by grind)
+
+/-- Falsum is absorbing for conjunction -/
+theorem bot_conj_absorb {A : Proposition Atom} : Equiv (A.conj bot) bot :=
+  equiv_iff.mpr ⟨botConjAbsorb⟩
+
+/-- Falsum is neutral for disjunction -/
+def botDisjNeutral {A : Proposition Atom} : Proposition.equiv (A.disj bot) A := by
+  constructor
+  · apply disjE (A := A) (B := bot)
+    · exact ax' (by grind)
+    · exact ax' (by grind)
+    · apply botE
+      exact ax' (by grind)
+  · apply disjI₁
+    exact ax' (by grind)
+
+/-- Falsum is neutral for disjunction -/
+theorem bot_disj_neutral {A : Proposition Atom} : Equiv (A.disj bot) A :=
+  equiv_iff.mpr ⟨botDisjNeutral⟩
+
+end NJ
+
+end IPL
